mark-and-sweep/spec/GC.Spec.ChunkedMajorGC.Graph.fsti
@@ -55,6 +55,17 @@ val chunked_major_successors_preserved
   (x: obj_addr)
   : prop
 
+val chunked_major_successors_preserved_elim
+  (mh_init: MH.major_heap)
+  (mh_final: MH.major_heap)
+  (x: obj_addr)
+  : Lemma
+      (requires chunked_major_successors_preserved mh_init mh_final x)
+      (ensures
+        forall (y: obj_addr).
+          chunked_major_edge mh_init x y <==>
+          chunked_major_edge mh_final x y)
+
 val chunked_major_vertex_single_chunk_compat
   (g: heap)
   (x: obj_addr)
